Aligned decoders for strings.

src/Narcissus/BinLib/AlignedString.v
@@ -22,6 +22,8 @@ Require Import
         Fiat.Narcissus.Formats.AsciiOpt
         Fiat.Narcissus.BinLib.AlignedByteString
         Fiat.Narcissus.BinLib.AlignWord
+        Fiat.Narcissus.BinLib.AlignedEncodeMonad
+        Fiat.Narcissus.BinLib.AlignedDecodeMonad
         Fiat.Common.IterateBoundedIndex
         Fiat.Common.Tactics.CacheStringConstant.
 
@@ -166,5 +168,281 @@ Section AlignedList.
                               `(s, b', cd') <- align_decode_string_with_term_char term_char v' cd;
                               Some (String (ascii_of_N (wordToN c)) s, b', cd')
     end.
+
+  Definition asciiToWord (a : ascii) : word 8 :=
+    match a with
+    | Ascii b0 b1 b2 b3 b4 b5 b6 b7 =>WS b0 (WS b1 (WS b2 (WS b3 (WS b4 (WS b5 (WS b6 (WS b7 WO)))))))
+    end.
+
+  Fixpoint AlignedEncodeString'
+           (sz : nat)
+           v
+           idx
+           (s : string)
+           env
+    : option (ByteBuffer.t sz * nat * CacheFormat) :=
+      match s with
+      | EmptyString => if Coq.Init.Nat.ltb idx (S sz) then @ReturnAlignedEncodeM _ string sz v idx EmptyString env else None
+      | String a s' => Ifopt (SetCurrentBytes (sz := 1) v idx (asciiToWord a) env) as a' Then
+                                                                AlignedEncodeString' sz (fst (fst a'))
+                                                              (snd (fst a'))
+                                                              s' (snd a')
+                                                              Else None
+    end.
+
+  Lemma asciiToWord_eq :
+    forall a,
+      (NToWord 8 (N_of_ascii a)) = asciiToWord a.
+  Proof.
+    destruct a; simpl.
+    destruct b; destruct b0; destruct b1; destruct b2;
+      destruct b3; destruct b4; destruct b5; destruct b6;
+      simpl; eauto.
+  Qed.
+
+  Definition AlignedEncodeString
+    : forall sz, AlignedEncodeM (S := string) sz := AlignedEncodeString'.
+
+  Lemma CorrectAlignedEncoderForFormatString
+    : CorrectAlignedEncoder format_string AlignedEncodeString.
+  Proof.
+    unfold CorrectAlignedEncoder; intros.
+    eexists (fix EncodeString (s : string) env :=
+               match s with
+               | EmptyString => Some (mempty, env)
+               | String a s' => `(t1, env') <- Some (WordOpt.encode_word (asciiToWord a) env);
+                             `(t2, env'') <- EncodeString s' env';
+                             Some (mappend t1 t2, env'')
+               end); split; [ split | split ].
+    - revert env; induction s; intros; simpl; eauto.
+      + injections; reflexivity.
+      + simpl in H.
+        unfold Bind2.
+        unfold format_ascii.
+        unfold WordOpt.format_word; simpl.
+        destruct ((fix EncodeString (s : string) (env : CacheFormat) {struct s} :
+                            option (ByteString * CacheFormat) :=
+                          match s with
+                          | ""%string => Some (ByteString_id, env)
+                          | String a s' =>
+                              `(t2, env'') <- EncodeString s' (addE env 8);
+                              Some
+                                (ByteString_enqueue_ByteString
+                                   (WordOpt.encode_word' 8 (asciiToWord a) ByteString_id) t2, env'')
+                          end)) eqn: ?; simpl in H; try discriminate.
+        destruct p; injections.
+        rewrite refineEquiv_bind_unit, IHs, refineEquiv_bind_unit; eauto.
+        simpl; rewrite asciiToWord_eq.
+        reflexivity.
+    - revert env; induction s; intros; simpl; eauto; try discriminate.
+      simpl in H.
+      destruct ((fix EncodeString (s : string) (env : CacheFormat) {struct s} :
+                            option (ByteString * CacheFormat) :=
+                          match s with
+                          | ""%string => Some (ByteString_id, env)
+                          | String a s' =>
+                              `(t2, env'') <- EncodeString s' (addE env 8);
+                              Some
+                                (ByteString_enqueue_ByteString
+                                   (WordOpt.encode_word' 8 (asciiToWord a) ByteString_id) t2, env'')
+                          end)) eqn: ?; simpl in H; try discriminate.
+      destruct p; injections; try discriminate.
+      unfold Bind2.
+      unfold format_ascii.
+      intro; computes_to_inv.
+      unfold WordOpt.format_word in H0; computes_to_inv; subst.
+      eapply IHs; eauto.
+    - induction s; intros; simpl; eauto.
+      + injections; reflexivity.
+      + simpl in *.
+        destruct ((fix EncodeString (s : string) (env : CacheFormat) {struct s} :
+                     option (ByteString * CacheFormat) :=
+                     match s with
+                     | ""%string => Some (ByteString_id, env)
+                     | String a s' =>
+                       `(t2, env'') <- EncodeString s' (addE env 8);
+                       Some
+                         (ByteString_enqueue_ByteString
+                            (WordOpt.encode_word' 8 (asciiToWord a) ByteString_id) t2, env'')
+                     end)) eqn: ?; simpl in H; try discriminate.
+        destruct p; injections; try discriminate.
+        eapply IHs in Heqo.
+        erewrite padding_ByteString_enqueue_ByteString, Heqo.
+        destruct a; reflexivity.
+    - unfold EncodeMEquivAlignedEncodeM; intros.
+      generalize (le_refl (String.length s)); remember (String.length s) eqn: s_eq; rewrite s_eq at 1; clear s_eq.
+      revert s env idx. induction n; intros ? ? ? le_s.
+      + destruct s; simpl in le_s; try solve [inversion le_s].
+        repeat apply conj; intros.
+        * injections; simpl in v; pattern v; apply case0; simpl.
+          setoid_rewrite (proj2 (PeanoNat.Nat.ltb_lt idx (S idx + m))); try Omega.omega.
+          eexists _; split.
+          revert v1; rewrite <- (plus_n_O idx); intro; reflexivity.
+          pose proof mempty_left as H'; simpl in H'; rewrite H', build_aligned_ByteString_append;
+            reflexivity.
+        * injections; rewrite length_ByteString_ByteString_id in H0.
+          unfold AlignedEncodeString; simpl.
+          destruct (NPeano.Nat.ltb idx (S numBytes')) eqn: ?; eauto.
+          apply PeanoNat.Nat.ltb_lt in Heqb; Omega.omega.
+        * injections; simpl in H0; congruence.
+        * discriminate.
+      + destruct s; simpl in le_s; try solve [inversion le_s].
+        * repeat apply conj; intros.
+          -- injections; simpl in v; pattern v; apply case0; simpl.
+             setoid_rewrite (proj2 (PeanoNat.Nat.ltb_lt idx (S idx + m))); try Lia.lia.
+             eexists _; split.
+             revert v1; rewrite <- (plus_n_O idx); intro; reflexivity.
+             pose proof mempty_left as H'; simpl in H'; rewrite H', build_aligned_ByteString_append;
+               reflexivity.
+          -- injections; rewrite length_ByteString_ByteString_id in H0.
+             unfold AlignedEncodeString; simpl.
+             destruct (NPeano.Nat.ltb idx (S numBytes')) eqn: ?; eauto.
+             apply PeanoNat.Nat.ltb_lt in Heqb; Omega.omega.
+          -- injections; simpl in H0; congruence.
+          -- discriminate.
+        * apply le_S_n in le_s.
+          intuition.
+          simpl in H.
+          -- destruct ((fix EncodeString (s : string) (env : CacheFormat) {struct s} :
+                          option (ByteString * CacheFormat) :=
+                          match s with
+                          | ""%string => Some (ByteString_id, env)
+                          | String a s' =>
+                            `(t2, env'') <- EncodeString s' (addE env 8);
+                            Some
+                              (ByteString_enqueue_ByteString
+                                 (WordOpt.encode_word' 8 (asciiToWord a) ByteString_id) t2, env'')
+                          end)) eqn: ?; simpl in H; try discriminate.
+             destruct p; injections; try discriminate.
+             simpl in *.
+             eapply IHn in le_s.
+             intuition.
+             eapply H in Heqo.
+             destruct Heqo; intuition.
+             eexists _.
+             intuition.
+             (*unfold SetCurrentByte; simpl.
+             simpl.
+
+
+             simpl in H2.
+          eapply H.
+          assert ((forall (s : A * {As : list A & le (length As) n} ) (env : CacheFormat) (t : ByteString) (env' : CacheFormat),
+                      (projT1 X ∘ fst) s env = Some (t, env') -> padding t = 0)) as H'.
+          { destruct X; clear IHn; simpl in *; intuition eauto. }
+          assert (EncodeMEquivAlignedEncodeM (projT1 X ∘ fst)
+                                             (fun (sz : nat) (t : ByteBuffer.t sz) (idx : nat)
+                                                  (s : A * {As : list A & le (length As) n})
+                                                  (env : CacheFormat) => encode_A sz t idx (fst s) env)) as H''.
+          { destruct X; clear IHn; simpl in *; intuition eauto.
+            unfold EncodeMEquivAlignedEncodeM; intros ? [? ?] ?; unfold Basics.compose; simpl.
+            apply H2; eauto. }
+          assert (EncodeMEquivAlignedEncodeM (S := A * {As : list A & le (length As) n})
+                    ((fix AlignedEncodeList (As : list A)
+                          (env : CacheFormat) {struct As} : option (ByteString * CacheFormat) :=
+                        match As with
+                        | [] => Some (mempty, env)
+                        | a :: As' => `(t1, env') <- projT1 X a env;
+                                      `(t2, env'') <- AlignedEncodeList As' env';
+                                      Some (mappend t1 t2, env'')
+                        end) ∘ (@projT1 _ _) ∘ snd )
+                    (fun (sz : nat) (t : ByteBuffer.t sz) (idx : nat)
+                         (s : A * {As : list A & le (length As) n}) (env : CacheFormat) =>
+                       AlignedEncodeList encode_A sz t idx (projT1 (snd s)) env)) as H'''.
+          { unfold EncodeMEquivAlignedEncodeM; intros ? [? [? ?] ] ?; simpl; eauto. }
+          apply le_S_n in le_s.
+        pose proof (Append_EncodeMEquivAlignedEncodeM _
+                                                      _
+                                                      _
+                                                      _
+                                                      H' H'' H''' env (a, existT _ s le_s) idx); clear H' H'' H'''.
+        intuition.
+  Qed. *)
+  Admitted.
+
+  Lemma CorrectAlignedEncoderForFormatStringTerm
+        term_char
+    : CorrectAlignedEncoderFor (format_string_with_term_char term_char).
+  Proof.
+    eexists.
+    eapply refine_CorrectAlignedEncoder with (format' := FMapFormat.Projection_Format format_string  (fun s => s ++ String term_char "")%string).
+    - split; intros.
+      + unfold format_string_with_term_char, FMapFormat.Projection_Format, FMapFormat.Compose_Format.
+        intros [? ?] ?.
+        rewrite unfold_computes in H; destruct H; intuition; subst; eauto.
+      + intros.
+        intros ?; eapply H.
+        unfold format_string_with_term_char in H0;
+          unfold FMapFormat.Projection_Format, FMapFormat.Compose_Format.
+        apply unfold_computes; eexists _; eauto.
+    - eapply CorrectAlignedEncoderProjection.
+      eapply CorrectAlignedEncoderForFormatString.
+  Defined.
+
+  Definition AlignedEncoderForFormatStringTerm
+             term_char
+    :=
+      Eval simpl in projT1 (CorrectAlignedEncoderForFormatStringTerm term_char).
+
+  Lemma CorrectAlignedEncoderFormatStringTerm
+        term_char
+    : CorrectAlignedEncoder (format_string_with_term_char term_char)
+                            (AlignedEncoderForFormatStringTerm term_char).
+  Proof.
+    apply (projT2 (CorrectAlignedEncoderForFormatStringTerm _)).
+  Qed.
+
+  Fixpoint StringAlignedDecodeM {m}
+           (term_char : word 8)
+           (n : nat)
+    : AlignedDecodeM string m :=
+    match n with
+    | 0 => ThrowAlignedDecodeM
+    | S n' => BindAlignedDecodeM GetCurrentByte
+                                 (fun c => if (weqb c term_char)
+                                           then ReturnAlignedDecodeM EmptyString
+                                           else BindAlignedDecodeM (StringAlignedDecodeM term_char n')
+                                                                   (fun s => ReturnAlignedDecodeM (String (ascii_of_N (wordToN c)) s)))
+    end%AlignedDecodeM%list.
+
+  Lemma AlignedDecodeStringM {C : Type}
+        (term_word : word 8)
+        (term_char : ascii)
+    : forall (t : string -> DecodeM (C * _) ByteString)
+             (t' : string -> forall {numBytes}, AlignedDecodeM C numBytes),
+      ascii_of_N (wordToN term_word) = term_char ->
+      (forall b, DecodeMEquivAlignedDecodeM (t b) (@t' b))
+      -> DecodeMEquivAlignedDecodeM
+           (fun v cd => `(l, bs, cd') <- decode_string_with_term_char term_char v cd;
+                          t l bs cd')
+           (fun numBytes => l <- @StringAlignedDecodeM numBytes term_word numBytes;
+           t' l)%AlignedDecodeM%list.
+  Proof.
+    intros.
+    (* unfold DecodeMEquivAlignedDecodeM; intuition.
+    eapply DecodeMEquivAlignedDecodeM_trans; simpl; intros.
+    2: reflexivity.
+    2: apply AlignedDecodeMEquiv_sym; etransitivity; [apply ReturnAlignedDecodeM_LeftUnit;
+                                                      reflexivity | reflexivity ].
+    eauto.
+    eapply DecodeMEquivAlignedDecodeM_trans; simpl; intros.
+    2: set_evars; erewrite !DecodeBindOpt2_assoc; subst_evars; higher_order_reflexivity.
+    2: apply AlignedDecodeMEquiv_sym; etransitivity; [apply BindAlignedDecodeM_assoc;
+                                                      reflexivity | higher_order_reflexivity ].
+    simpl.
+    eapply Bind_DecodeMEquivAlignedDecodeM; intros.
+    eauto.
+    eapply DecodeMEquivAlignedDecodeM_trans; simpl; intros.
+    2: set_evars; erewrite !DecodeBindOpt2_assoc; subst_evars; higher_order_reflexivity.
+    2: apply AlignedDecodeMEquiv_sym; etransitivity; [apply BindAlignedDecodeM_assoc;
+                                                      reflexivity | higher_order_reflexivity ].
+    simpl.
+    eapply IHn; eauto.
+    intros.
+    eapply DecodeMEquivAlignedDecodeM_trans; simpl; intros.
+    2: higher_order_reflexivity.
+    2: apply AlignedDecodeMEquiv_sym; etransitivity; [eapply ReturnAlignedDecodeM_LeftUnit | higher_order_reflexivity].
+    eapply H0. *)
+  Admitted.
 
 End AlignedList.
